

$$⑥ y = 5\sqrt{x} \quad y' = \frac{5}{2\sqrt{x}}$$

$$\text{at } m = \frac{-1}{\frac{5}{4}} = \frac{-4}{5}$$

$$y - 10 = \frac{-4}{5}(x - 4)$$

$$\text{Normal } y - 10 = \frac{-4}{5}(x - 4)$$

$$Q = \left(\frac{33}{2}, 10\right)$$

$$⑦ y' = 5 - 24x^{-3} = 5 - \frac{24}{x^3}$$

$$⑧ y'(2) = 5 - \frac{24}{2} = 5 - 3 = 2$$

$$y - 13 = \frac{-1}{2}(x - 2)$$

$$x - 26 = 26$$

$$\boxed{x = 28}$$

$$\underline{\underline{(28, 0)}}$$

TO 2
 1. 150 STEP 2

$$\textcircled{1} \frac{3x^5 - 7}{4x}$$

$$y = \frac{3}{4}x^4 - \frac{7}{4}x^{-1}$$

$$\frac{dy}{dx} = 3x^3 + \frac{7}{4x^2}$$

$$\textcircled{2} y = \frac{8}{4x-5} \quad y' = 8 \times \frac{-4}{(4x-5)^2} = \frac{-32}{(4x-5)^2}$$

$$y'(2) = \frac{-32}{9}$$

$$\textcircled{3} y = 3x^3 - 3x^2 + x - 7$$

$$y' = 9x^2 - 6x + 1$$

$$x = \frac{6}{18} = \frac{1}{3}$$

$$y'(\frac{1}{3}) = 9(\frac{1}{9}) - 6(\frac{1}{3}) + 1 = 1 - 2 + 1 = 0$$

$$y' \geq 0$$

$$\textcircled{4} y = (3-5x)^3 - 2x$$

$$\frac{dy}{dx} = 3(3-5x)^2 \times (-5) - 2 = -15(3-5x)^2 - 2$$

$$\frac{d^2y}{dx^2} = -15 \times 2(3-5x) \times (-5) = 150(3-5x)$$

$$\textcircled{5} y = \frac{15}{x^2 - 2x} = 15(x^2 - 2x)^{-1}$$

$$y' = -15(2x - 2)(x^2 - 2x)^{-2} = \frac{-30(x-1)}{(x^2 - 2x)^2}$$

$$y'(5) = \frac{-120}{225} = \frac{-8}{15}$$